Uncurried primitives and simplified weak bisimilarity
- As Jeremy Yallop suggested, I change the semantics of the primitives
pair, proj1, proj2, fork, ret to offer them as base primitives. This
change has been filtered through to proofs and the extracted code. The
extracted code was then evaluated and surprisingly it worked on the
first run. The lack of currying actually reduced the number of errors
made by the extraction plugin.

- I have simiplified the weak bisimilarity based on the remark in
Sangiorgi's comment in his " The problem of “Weak Bisimulation up to” "
paper: I have proven that the single step based weak bisimilarity is
equivalent to the original and then went on to prove the monadic
properties, part of fork commutativity (only side effects, not the
switch yet) in 70 lines. This reduced the proof substantially as I did
not have to build my own inversion Lemmas, and push lemmas and I could
just use the built in ones. (To put it in perspective, it used to be
about 3000 lines long).

Evaluation/Deleuze/sugarcube.ml
@@ -11,7 +11,7 @@ let ( >>= ) a b = E_bind (a, b)
 
 let app a b = E_apply (a, b)
 
-let fork a b = app ( app (E_constant CONST_fork) a ) b
+let fork a b = E_fork (a, b)
 
 let func v t e = E_function (v, t, e)
 
@@ -19,16 +19,16 @@ let case e1 x1 e2 x2 e3 = E_case (e1, x1, e2, x2, e3)
 
 let fix e = E_fix e
 
-let pair a b = (app (app (E_constant CONST_pair) a) b)
+let pair a b = E_inpair (a, b)
 
-let ret a = app (E_constant CONST_ret) a
+let ret a = E_ret a
 
-let proj1 a = app (E_constant CONST_proj1) a
-let proj2 a = app (E_constant CONST_proj2) a
+let proj1 a = E_proj1 a
+let proj2 a = E_proj2 a
 
 let rec v_expr = function
 | E_ident value_name5 -> value_name5::[]
-| E_constant constant5 -> []
+| E_unit -> []
 | E_apply (expr5, expr') -> append (v_expr expr5) (v_expr expr')
 | E_bind (expr5, expr') -> append (v_expr expr5) (v_expr expr')
 | E_function (value_name5, typexpr5, expr5) -> append (v_expr expr5) (value_name5::[])
@@ -36,14 +36,21 @@ let rec v_expr = function
 | E_comp e -> []
 | E_live_expr e -> v_expr e
 | E_pair (e, e') -> append (v_expr e) (v_expr e')
+| E_inpair (e, e') -> append (v_expr e) (v_expr e')
+| E_proj1 e -> v_expr e
+| E_proj2 e -> v_expr e
+| E_fork (e, e') -> append (v_expr e) (v_expr e')
+| E_ret e -> (v_expr e)
 | E_taggingleft e -> v_expr e
 | E_taggingright e -> v_expr e
 | E_case (e1, x1, e2, x2, e3) ->
   append (v_expr e1) (append (v_expr e2) (v_expr e3))
 
-let cunit = E_constant CONST_unit
 
-let tunit = TE_constants TC_unit
+
+let cunit = E_unit
+
+let tunit = TE_unit
 
 let tfun a b = TE_arrow(a,b)
 
