combinedPieces.ml
@@ -1,4 +1,3 @@
-(** commons:  **)
 type value_name = int
 
 (** val eq_value_name : value_name -> value_name -> bool **)
@@ -21,44 +20,281 @@ let rec eq_value_name n y0 =
       y0)
     n
 
-type ident = int
-
-type typvar =
-  ident
-  (* singleton inductive, whose constructor was TV_ident *)
-
-type typconst =
-| TC_unit
-
 type typexpr =
-| TE_constants of typconst
-| TE_var of typvar
+| TE_unit
 | TE_arrow of typexpr * typexpr
 | TE_prod of typexpr * typexpr
 | TE_concurrent of typexpr
 | TE_sum of typexpr * typexpr
 
-type constant =
-| CONST_ret
-| CONST_fork
-| CONST_unit
-| CONST_pair
-| CONST_proj1
-| CONST_proj2
-
 type expr =
 | E_ident of value_name
-| E_constant of constant
+| E_unit
 | E_apply of expr * expr
 | E_bind of expr * expr
 | E_function of value_name * typexpr * expr
 | E_fix of expr
-| E_comp of (unit -> expr)
+| E_comp of (unit -> expr)                                                   (* modified placeholder *)
 | E_live_expr of expr
 | E_pair of expr * expr
+| E_inpair of expr * expr
+| E_proj1 of expr
+| E_proj2 of expr
+| E_fork of expr * expr
+| E_ret of expr
 | E_taggingleft of expr
 | E_taggingright of expr
 | E_case of expr * value_name * expr * value_name * expr
+
+(** val list_mem : ('a1 -> 'a1 -> bool) -> 'a1 -> 'a1 list -> bool **)
+
+let rec list_mem eq x = function
+| [] -> false
+| h::t -> if eq h x then true else list_mem eq x t
+
+(** val subst_expr : expr -> value_name -> expr -> expr **)
+
+let rec subst_expr e_5 x_5 = function
+| E_ident value_name5 ->
+  if eq_value_name value_name5 x_5 then e_5 else E_ident value_name5
+| E_unit -> E_unit
+| E_apply (expr5, expr') ->
+  E_apply ((subst_expr e_5 x_5 expr5), (subst_expr e_5 x_5 expr'))
+| E_bind (expr5, expr') ->
+  E_bind ((subst_expr e_5 x_5 expr5), (subst_expr e_5 x_5 expr'))
+| E_function (value_name5, typexpr5, expr5) ->
+  E_function (value_name5, typexpr5,
+    (if list_mem eq_value_name x_5 (value_name5::[])
+     then expr5
+     else subst_expr e_5 x_5 expr5))
+| E_fix e -> E_fix (subst_expr e_5 x_5 e)
+| E_comp e -> E_comp (subst_expr e_5 x_5 e)                                      (* this substitution should not occur! *)
+| E_live_expr e -> E_live_expr (subst_expr e_5 x_5 e)
+| E_pair (e, e') -> E_pair ((subst_expr e_5 x_5 e), (subst_expr e_5 x_5 e'))
+| E_inpair (e, e') ->
+  E_inpair ((subst_expr e_5 x_5 e), (subst_expr e_5 x_5 e'))
+| E_proj1 e -> E_proj1 (subst_expr e_5 x_5 e)
+| E_proj2 e -> E_proj2 (subst_expr e_5 x_5 e)
+| E_fork (e, e') -> E_fork ((subst_expr e_5 x_5 e), (subst_expr e_5 x_5 e'))
+| E_ret e -> E_ret (subst_expr e_5 x_5 e)
+| E_taggingleft e -> E_taggingleft (subst_expr e_5 x_5 e)
+| E_taggingright e -> E_taggingright (subst_expr e_5 x_5 e)
+| E_case (e1, x1, e2, x2, e3) ->
+  E_case ((subst_expr e_5 x_5 e1), x1, (subst_expr e_5 x_5 e2), x2,
+    (subst_expr e_5 x_5 e3))
+
+(** val xis_value_of_expr : expr -> bool **)
+
+let rec xis_value_of_expr = function
+| E_unit -> true
+| E_function (value_name5, typexpr5, expr5) -> true
+| E_live_expr e -> true
+| E_pair (e, e') ->
+  if xis_value_of_expr e then xis_value_of_expr e' else false
+| E_taggingleft e -> xis_value_of_expr e
+| E_taggingright e -> xis_value_of_expr e
+| _ -> false
+
+(** val xJO_red12 : expr -> selectstar -> expr **)
+
+type selectstar = | Seq of select * (unit -> selectstar)  (* modified coinductive datatype to be lazy *)
+
+
+let rec xJO_red12 p1 p2 =
+  match (p1, p2) with
+  | (E_apply (E_function (x, t, e), v), s) ->
+    (match xis_value_of_expr v with
+     | true -> subst_expr v x e
+     | false -> E_apply (E_function (x, t, e), (xJO_red12 v s)))
+  | (E_ret v, s) ->
+    (match xis_value_of_expr v with
+     | true -> E_live_expr v
+     | false ->
+       (match xJO_red12 v s with
+        | v' -> E_ret v'
+        | _ -> assert false (*  *))
+    (* | _ -> assert false (*  *) *))
+  | (E_bind (E_live_expr e, e''), s) ->
+    (match xis_value_of_expr e with
+     | false ->
+       (match xJO_red12 e s with
+        | e' -> E_bind ((E_live_expr e'), e'')
+        | _ -> assert false (*  *))
+     | true -> E_apply (e'', e)
+     | _ -> assert false (*  *))
+  | (E_bind (e, e''), s) ->
+    (match xis_value_of_expr e with
+     | false ->
+       (match xJO_red12 e s with
+        | e' -> E_bind (e', e'')
+        | _ -> assert false (*  *))
+     | _ -> assert false (*  *))
+  | (E_inpair (v, v'), s) ->
+    (match xis_value_of_expr v with
+     | true ->
+       (match xis_value_of_expr v' with
+        | true -> E_pair (v, v')
+        | false ->
+          (match xJO_red12 v' s with
+           | v'' -> E_inpair (v, v'')
+           | _ -> assert false (*  *))
+        | _ -> assert false (*  *))
+     | false ->
+       (match xJO_red12 v s with
+        | v'' -> E_inpair (v'', v')
+        | _ -> assert false (*  *))
+     | _ -> assert false (*  *))
+  | (E_comp e, s) -> (e ())
+  | (E_proj1 E_pair (v, v'), s) ->
+    (match xis_value_of_expr v' with
+     | true ->
+       (match xis_value_of_expr v with
+        | true -> v
+        | _ -> assert false (*  *))
+     | false -> E_proj1 (xJO_red12 (E_pair (v, v')) s))            (* combine the reduce and do *)
+  | (E_proj2 E_pair (v, v'), s) ->
+    (match xis_value_of_expr v' with
+     | true ->
+       (match xis_value_of_expr v with
+        | true -> v'
+        | _ -> assert false (*  *))
+     | false -> E_proj2 (xJO_red12 (E_pair (v, v')) s))             (* combine the reduce and do *)
+ | (E_fork (E_live_expr e, E_live_expr e'), Seq (S_First, s)) ->
+    (match xis_value_of_expr e with                                       (* reordered unsafe assumption *)
+     | false ->
+       (match xis_value_of_expr e' with
+        | false ->
+          (match xJO_red12 e (s ()) with                                          (* Added code to use selecstar *)
+           | e'' -> E_fork ((E_live_expr e''), (E_live_expr e'))
+           | _ -> assert false (*  *))
+        | true -> E_live_expr (E_taggingright (E_pair ((E_live_expr e), e'))))                                       (* Fold in forkdeath 2 *)
+     | true -> E_live_expr (E_taggingleft (E_pair (e, (E_live_expr e')))))                                          (* Fold in forkdeath 1 *)
+  | (E_fork (E_live_expr e, E_live_expr e'), Seq (S_Second, s)) ->
+    (match xis_value_of_expr e'  with                                                        (* reordered unsafe assumption *)
+     | false ->
+       (match xis_value_of_expr e with
+        | false ->
+          (match xJO_red12 e' (s ()) with                                        (* Added code to use selecstar *)
+           | e'' -> E_fork ((E_live_expr e), (E_live_expr e''))
+           | _ -> assert false (*  *))
+        | true -> E_live_expr (E_taggingleft (E_pair (e, (E_live_expr e')))))                                 (* Fold in forkdeath 1 *)
+     | true -> E_live_expr (E_taggingright (E_pair ((E_live_expr e), e'))))                                   (* Fold in forkdeath 2 *)
+ (* | (E_fork (E_live_expr v, E_live_expr e), s) ->
+    (match xis_value_of_expr e with
+     | true -> E_live_expr (E_taggingleft (E_pair (v, (E_live_expr e))))                       (* Folded *)
+     | _ -> assert false (*  *)) *)
+  | (E_fork (e, e'), s) ->
+    (match xis_value_of_expr e with
+     | false ->
+       (match xJO_red12 e s with
+        | e'' -> E_fork (e'', e')
+        | _ -> assert false (*  *))
+     | true ->
+       (match xis_value_of_expr e' with                                                          (* reordered unsafe assumption *)
+        | false ->
+          (match xJO_red12 e' s with
+           | e'' -> E_fork (e, e'')
+           | _ -> assert false (*  *))
+        | _ -> assert false (*  *))
+     | _ -> assert false (*  *))
+ (*  | (E_fork (E_live_expr e, E_live_expr v'), s) ->
+    (match xis_value_of_expr v' with
+     | true -> E_live_expr (E_taggingright (E_pair ((E_live_expr e), v')))                      (* Folded *)
+     | _ -> assert false (*  *)) *)
+  | (E_apply (e, e'), s) ->
+    (match xis_value_of_expr e with
+     | false ->
+       (match xJO_red12 e s with
+        | e'' -> E_apply (e'', e')
+        | _ -> assert false (*  *))
+     | true ->
+       (match xJO_red12 e' s with
+        | e'' -> E_apply (e, e'')
+        | _ -> assert false (*  *))
+     | _ -> assert false (*  *))
+  | (E_fix E_function (x, t, e), s) ->
+    subst_expr (E_fix (E_function (x, t, e))) x e
+  | (E_fix e, s) ->
+    (match xJO_red12 e s with
+     | e' -> E_fix e'
+     | _ -> assert false (*  *))
+  | (E_pair (e, e''), s) ->
+    (match xis_value_of_expr e with
+     | false ->
+       (match xJO_red12 e s with
+        | e' -> E_pair (e', e'')
+        | _ -> assert false (*  *))
+     | true ->
+       (match xJO_red12 e'' s with
+        | e' -> E_pair (e, e')
+        | _ -> assert false (*  *))
+     | _ -> assert false (*  *))
+  | (E_taggingleft e, s) ->
+    (match xJO_red12 e s with
+     | e' -> E_taggingleft e'
+     | _ -> assert false (*  *))
+  | (E_taggingright e, s) ->
+    (match xJO_red12 e s with
+     | e' -> E_taggingright e'
+     | _ -> assert false (*  *))
+  | (E_case (E_taggingleft v, x, e, x', e'), s) ->
+    (match xis_value_of_expr v with
+     | true -> subst_expr v x e
+     | _ -> assert false (*  *))
+  | (E_case (E_taggingright v, x, e, x', e'), s) ->
+    (match xis_value_of_expr v with
+     | true -> subst_expr v x' e'
+     | _ -> assert false (*  *))
+  | (E_case (e, x, e'', x', e'''), s) ->
+    (match xJO_red12 e s with
+     | e' ->
+       (match xis_value_of_expr e with
+        | false -> E_case (e', x, e'', x', e''')
+        | _ -> assert false (*  *))
+     | _ -> assert false (*  *))
+  | _ -> assert false (*   *))
+
+
+(*
+type value_name = int
+
+type typexpr =
+| TE_unit
+| TE_arrow of typexpr * typexpr
+| TE_prod of typexpr * typexpr
+| TE_concurrent of typexpr
+| TE_sum of typexpr * typexpr
+
+type expr =
+| E_ident of value_name
+| E_unit
+| E_apply of expr * expr
+| E_bind of expr * expr
+| E_function of value_name * typexpr * expr
+| E_fix of expr
+| E_comp of expr
+| E_live_expr of expr
+| E_pair of expr * expr
+| E_inpair of expr * expr
+| E_proj1 of expr
+| E_proj2 of expr
+| E_fork of expr * expr
+| E_ret of expr
+| E_taggingleft of expr
+| E_taggingright of expr
+| E_case of expr * value_name * expr * value_name * expr
+
+(** val xis_value_of_expr : expr -> bool **)
+
+let rec xis_value_of_expr = function
+| E_unit -> true
+| E_function (value_name5, typexpr5, expr5) -> true
+| E_live_expr e -> true
+| E_pair (e, e') ->
+  if xis_value_of_expr e then xis_value_of_expr e' else false
+| E_taggingleft e -> xis_value_of_expr e
+| E_taggingright e -> xis_value_of_expr e
+| _ -> false
 
 type select =
 | S_First
@@ -75,7 +311,7 @@ let rec list_mem eq x = function
 let rec subst_expr e_5 x_5 = function
 | E_ident value_name5 ->
   if eq_value_name value_name5 x_5 then e_5 else E_ident value_name5
-| E_constant constant5 -> E_constant constant5
+| E_unit -> E_unit
 | E_apply (expr5, expr') ->
   E_apply ((subst_expr e_5 x_5 expr5), (subst_expr e_5 x_5 expr'))
 | E_bind (expr5, expr') ->
@@ -86,48 +322,21 @@ let rec subst_expr e_5 x_5 = function
      then expr5
      else subst_expr e_5 x_5 expr5))
 | E_fix e -> E_fix (subst_expr e_5 x_5 e)
-| E_comp e -> E_comp (e)                                                    (* By no means should substitution happen here *)
+| E_comp e -> E_comp (subst_expr e_5 x_5 e)
 | E_live_expr e -> E_live_expr (subst_expr e_5 x_5 e)
 | E_pair (e, e') -> E_pair ((subst_expr e_5 x_5 e), (subst_expr e_5 x_5 e'))
+| E_inpair (e, e') ->
+  E_inpair ((subst_expr e_5 x_5 e), (subst_expr e_5 x_5 e'))
+| E_proj1 e -> E_proj1 (subst_expr e_5 x_5 e)
+| E_proj2 e -> E_proj2 (subst_expr e_5 x_5 e)
+| E_fork (e, e') -> E_fork ((subst_expr e_5 x_5 e), (subst_expr e_5 x_5 e'))
+| E_ret e -> E_ret (subst_expr e_5 x_5 e)
 | E_taggingleft e -> E_taggingleft (subst_expr e_5 x_5 e)
 | E_taggingright e -> E_taggingright (subst_expr e_5 x_5 e)
 | E_case (e1, x1, e2, x2, e3) ->
   E_case ((subst_expr e_5 x_5 e1), x1, (subst_expr e_5 x_5 e2), x2,
     (subst_expr e_5 x_5 e3))
 
-(** val xis_value_of_expr : expr -> bool **)
-
-let rec xis_value_of_expr = function
-| E_constant constant5 -> true
-| E_apply (expr5, expr') ->
-  (match expr5 with
-   | E_constant constant5 ->
-     (match constant5 with
-      | CONST_fork -> xis_value_of_expr expr'
-      | CONST_pair -> xis_value_of_expr expr'
-      | _ ->
-        (match expr5 with
-         | E_constant constant6 ->
-           (match constant6 with
-            | CONST_fork -> xis_value_of_expr expr'
-            | CONST_pair -> xis_value_of_expr expr'
-            | _ -> false)
-         | _ -> false))
-   | _ ->
-     (match expr5 with
-      | E_constant constant5 ->
-        (match constant5 with
-         | CONST_fork -> xis_value_of_expr expr'
-         | CONST_pair -> xis_value_of_expr expr'
-         | _ -> false)
-      | _ -> false))
-| E_function (value_name5, typexpr5, expr5) -> true
-| E_live_expr expr5 -> true
-| E_pair (e, e') ->
-  if xis_value_of_expr e then xis_value_of_expr e' else false
-| E_taggingleft e -> xis_value_of_expr e
-| E_taggingright e -> xis_value_of_expr e
-| _ -> false
 
 
 (** val xJO_red12 : expr -> selectstar -> expr **)
@@ -272,6 +481,8 @@ let rec xJO_red12 p1 p2 =
         | _ -> assert false (*  *))
      | _ -> assert false (*  *))
   | _ -> assert false (*  *)
+
+*)
 (*
 let rec xJO_red12 p1 p2 =
   match (p1, p2) with
