mconbase.v
@@ -11,34 +11,18 @@ Proof.
   decide equality; auto with ott_coq_equality arith.
 Defined.
 Hint Resolve eq_value_name : ott_coq_equality.
-Definition ident := nat.
 Definition index := nat.
 
-Inductive typvar : Set := 
- | TV_ident (ident5:ident).
-
-Inductive typconst : Set := 
- | TC_unit : typconst.
-
 Inductive typexpr : Set := 
- | TE_constants (typconst5:typconst)
- | TE_var (typvar5:typvar)
+ | TE_unit : typexpr
  | TE_arrow (typexpr5:typexpr) (typexpr':typexpr)
  | TE_prod (typexpr5:typexpr) (typexpr':typexpr)
  | TE_concurrent (typexpr5:typexpr)
  | TE_sum (typexpr5:typexpr) (typexpr':typexpr).
 
-Inductive constant : Set := 
- | CONST_ret : constant
- | CONST_fork : constant
- | CONST_unit : constant
- | CONST_pair : constant
- | CONST_proj1 : constant
- | CONST_proj2 : constant.
-
 Inductive expr : Set := 
  | E_ident (value_name5:value_name)
- | E_constant (constant5:constant)
+ | E_unit : expr
  | E_apply (expr5:expr) (expr':expr)
  | E_bind (expr5:expr) (expr':expr)
  | E_function (value_name5:value_name) (typexpr5:typexpr) (expr5:expr)
@@ -46,6 +30,11 @@ Inductive expr : Set :=
  | E_comp (e:expr)
  | E_live_expr (e:expr)
  | E_pair (e:expr) (e':expr)
+ | E_inpair (e:expr) (e':expr)
+ | E_proj1 (e:expr)
+ | E_proj2 (e:expr)
+ | E_fork (e:expr) (e':expr)
+ | E_ret (e:expr)
  | E_taggingleft (e:expr)
  | E_taggingright (e:expr)
  | E_case (e1:expr) (x1:value_name) (e2:expr) (x2:value_name) (e3:expr).
@@ -61,25 +50,24 @@ Inductive select : Set :=
 Inductive G : Set := 
  | G_em : G
  | G_vn (G5:G) (value_name5:value_name) (typexpr5:typexpr).
-Lemma eq_typvar: forall (x y : typvar), {x = y} + {x <> y}.
-Proof.
-decide equality. apply eq_value_name.
-Defined.
-Hint Resolve eq_typvar : ott_coq_equality.
 
 (** subrules *)
 Fixpoint is_value_of_expr (e_5:expr) : Prop :=
   match e_5 with
   | (E_ident value_name5) => False
-  | (E_constant constant5) => (True)
- (* Manual change *)
-  | (E_apply expr5 expr') => match expr5 with | E_constant (CONST_fork) => is_value_of_expr (expr') | E_constant (CONST_pair) => is_value_of_expr (expr') | _ => False end  
+  | E_unit => (True)
+  | (E_apply expr5 expr') => False
   | (E_bind expr5 expr') => False
   | (E_function value_name5 typexpr5 expr5) => (True)
   | (E_fix e) => False
   | (E_comp e) => False
   | (E_live_expr e) => (True)
   | (E_pair e e') => ((is_value_of_expr e) /\ (is_value_of_expr e'))
+  | (E_inpair e e') => False
+  | (E_proj1 e) => False
+  | (E_proj2 e) => False
+  | (E_fork e e') => False
+  | (E_ret e) => False
   | (E_taggingleft e) => ((is_value_of_expr e))
   | (E_taggingright e) => ((is_value_of_expr e))
   | (E_case e1 x1 e2 x2 e3) => False
@@ -93,29 +81,12 @@ Fixpoint list_mem A (eq:forall a b:A,{a=b}+{a<>b}) (x:A) (l:list A) {struct l} :
 end.
 Implicit Arguments list_mem.
 
-Fixpoint list_assoc A B (eq:forall a b:A,{a=b}+{a<>b}) (x:A) (l:list (A*B)) {struct l} : option B :=
-  match l with
-  | nil => None
-  | cons (a,b) t => if (eq a x) then Some b else list_assoc A B eq x t
-end.
-Implicit Arguments list_assoc.
-
 
 (** substitutions *)
-Fixpoint tsubst_typexpr (sub:list (typvar*typexpr)) (t_6:typexpr) {struct t_6} : typexpr :=
-  match t_6 with
-  | (TE_constants typconst5) => TE_constants typconst5
-  | (TE_var typvar5) => (match list_assoc eq_typvar typvar5 sub with None => (TE_var typvar5) | Some t5 => t5 end)
-  | (TE_arrow typexpr5 typexpr') => TE_arrow (tsubst_typexpr sub typexpr5) (tsubst_typexpr sub typexpr')
-  | (TE_prod typexpr5 typexpr') => TE_prod (tsubst_typexpr sub typexpr5) (tsubst_typexpr sub typexpr')
-  | (TE_concurrent typexpr5) => TE_concurrent (tsubst_typexpr sub typexpr5)
-  | (TE_sum typexpr5 typexpr') => TE_sum (tsubst_typexpr sub typexpr5) (tsubst_typexpr sub typexpr')
-end.
-
 Fixpoint subst_expr (e_5:expr) (x_5:value_name) (e__6:expr) {struct e__6} : expr :=
   match e__6 with
   | (E_ident value_name5) => (if eq_value_name value_name5 x_5 then e_5 else (E_ident value_name5))
-  | (E_constant constant5) => E_constant constant5
+  | E_unit => E_unit 
   | (E_apply expr5 expr') => E_apply (subst_expr e_5 x_5 expr5) (subst_expr e_5 x_5 expr')
   | (E_bind expr5 expr') => E_bind (subst_expr e_5 x_5 expr5) (subst_expr e_5 x_5 expr')
   | (E_function value_name5 typexpr5 expr5) => E_function value_name5 typexpr5 (if list_mem eq_value_name x_5 (cons value_name5 nil) then expr5 else (subst_expr e_5 x_5 expr5))
@@ -123,43 +94,20 @@ Fixpoint subst_expr (e_5:expr) (x_5:value_name) (e__6:expr) {struct e__6} : expr
   | (E_comp e) => E_comp (subst_expr e_5 x_5 e)
   | (E_live_expr e) => E_live_expr (subst_expr e_5 x_5 e)
   | (E_pair e e') => E_pair (subst_expr e_5 x_5 e) (subst_expr e_5 x_5 e')
+  | (E_inpair e e') => E_inpair (subst_expr e_5 x_5 e) (subst_expr e_5 x_5 e')
+  | (E_proj1 e) => E_proj1 (subst_expr e_5 x_5 e)
+  | (E_proj2 e) => E_proj2 (subst_expr e_5 x_5 e)
+  | (E_fork e e') => E_fork (subst_expr e_5 x_5 e) (subst_expr e_5 x_5 e')
+  | (E_ret e) => E_ret (subst_expr e_5 x_5 e)
   | (E_taggingleft e) => E_taggingleft (subst_expr e_5 x_5 e)
   | (E_taggingright e) => E_taggingright (subst_expr e_5 x_5 e)
   | (E_case e1 x1 e2 x2 e3) => E_case (subst_expr e_5 x_5 e1) x1 (subst_expr e_5 x_5 e2) x2 (subst_expr e_5 x_5 e3)
-end.
-
-Fixpoint tsubst_expr (sub:list (typvar*typexpr)) (e_5:expr) {struct e_5} : expr :=
-  match e_5 with
-  | (E_ident value_name5) => E_ident value_name5
-  | (E_constant constant5) => E_constant constant5
-  | (E_apply expr5 expr') => E_apply (tsubst_expr sub expr5) (tsubst_expr sub expr')
-  | (E_bind expr5 expr') => E_bind (tsubst_expr sub expr5) (tsubst_expr sub expr')
-  | (E_function value_name5 typexpr5 expr5) => E_function value_name5 (tsubst_typexpr sub typexpr5) (tsubst_expr sub expr5)
-  | (E_fix e) => E_fix (tsubst_expr sub e)
-  | (E_comp e) => E_comp (tsubst_expr sub e)
-  | (E_live_expr e) => E_live_expr (tsubst_expr sub e)
-  | (E_pair e e') => E_pair (tsubst_expr sub e) (tsubst_expr sub e')
-  | (E_taggingleft e) => E_taggingleft (tsubst_expr sub e)
-  | (E_taggingright e) => E_taggingright (tsubst_expr sub e)
-  | (E_case e1 x1 e2 x2 e3) => E_case (tsubst_expr sub e1) x1 (tsubst_expr sub e2) x2 (tsubst_expr sub e3)
 end.
 
 Definition subst_redlabel (e5:expr) (x5:value_name) (rl5:redlabel) : redlabel :=
   match rl5 with
   | RL_tau => RL_tau 
   | (RL_labelled expr5) => RL_labelled (subst_expr e5 x5 expr5)
-end.
-
-Definition tsubst_redlabel (sub:list (typvar*typexpr)) (rl5:redlabel) : redlabel :=
-  match rl5 with
-  | RL_tau => RL_tau 
-  | (RL_labelled expr5) => RL_labelled (tsubst_expr sub expr5)
-end.
-
-Fixpoint tsubst_G (sub:list (typvar*typexpr)) (G_6:G) {struct G_6} : G :=
-  match G_6 with
-  | G_em => G_em 
-  | (G_vn G5 value_name5 typexpr5) => G_vn (tsubst_G sub G5) value_name5 (tsubst_typexpr sub typexpr5)
 end.
 
 (** library functions *)
@@ -172,36 +120,10 @@ Implicit Arguments list_minus.
 
 
 (** free variables *)
-Fixpoint ftv_typexpr (t5:typexpr) : list typvar :=
-  match t5 with
-  | (TE_constants typconst5) => nil
-  | (TE_var typvar5) => (cons typvar5 nil)
-  | (TE_arrow typexpr5 typexpr') => (app (ftv_typexpr typexpr5) (ftv_typexpr typexpr'))
-  | (TE_prod typexpr5 typexpr') => (app (ftv_typexpr typexpr5) (ftv_typexpr typexpr'))
-  | (TE_concurrent typexpr5) => ((ftv_typexpr typexpr5))
-  | (TE_sum typexpr5 typexpr') => (app (ftv_typexpr typexpr5) (ftv_typexpr typexpr'))
-end.
-
-Fixpoint ftv_expr (e_5:expr) : list typvar :=
-  match e_5 with
-  | (E_ident value_name5) => nil
-  | (E_constant constant5) => nil
-  | (E_apply expr5 expr') => (app (ftv_expr expr5) (ftv_expr expr'))
-  | (E_bind expr5 expr') => (app (ftv_expr expr5) (ftv_expr expr'))
-  | (E_function value_name5 typexpr5 expr5) => (app (ftv_typexpr typexpr5) (ftv_expr expr5))
-  | (E_fix e) => ((ftv_expr e))
-  | (E_comp e) => ((ftv_expr e))
-  | (E_live_expr e) => ((ftv_expr e))
-  | (E_pair e e') => (app (ftv_expr e) (ftv_expr e'))
-  | (E_taggingleft e) => ((ftv_expr e))
-  | (E_taggingright e) => ((ftv_expr e))
-  | (E_case e1 x1 e2 x2 e3) => (app (ftv_expr e1) (app (ftv_expr e2) (ftv_expr e3)))
-end.
-
 Fixpoint fv_expr (e_5:expr) : list value_name :=
   match e_5 with
   | (E_ident value_name5) => (cons value_name5 nil)
-  | (E_constant constant5) => nil
+  | E_unit => nil
   | (E_apply expr5 expr') => (app (fv_expr expr5) (fv_expr expr'))
   | (E_bind expr5 expr') => (app (fv_expr expr5) (fv_expr expr'))
   | (E_function value_name5 typexpr5 expr5) => ((list_minus eq_value_name (fv_expr expr5) (cons value_name5 nil)))
@@ -209,21 +131,14 @@ Fixpoint fv_expr (e_5:expr) : list value_name :=
   | (E_comp e) => ((fv_expr e))
   | (E_live_expr e) => ((fv_expr e))
   | (E_pair e e') => (app (fv_expr e) (fv_expr e'))
+  | (E_inpair e e') => (app (fv_expr e) (fv_expr e'))
+  | (E_proj1 e) => ((fv_expr e))
+  | (E_proj2 e) => ((fv_expr e))
+  | (E_fork e e') => (app (fv_expr e) (fv_expr e'))
+  | (E_ret e) => ((fv_expr e))
   | (E_taggingleft e) => ((fv_expr e))
   | (E_taggingright e) => ((fv_expr e))
   | (E_case e1 x1 e2 x2 e3) => (app (fv_expr e1) (app (fv_expr e2) (fv_expr e3)))
-end.
-
-Definition ftv_redlabel (rl5:redlabel) : list typvar :=
-  match rl5 with
-  | RL_tau => nil
-  | (RL_labelled expr5) => ((ftv_expr expr5))
-end.
-
-Fixpoint ftv_G (G_6:G) : list typvar :=
-  match G_6 with
-  | G_em => nil
-  | (G_vn G5 value_name5 typexpr5) => (app (ftv_G G5) (ftv_typexpr typexpr5))
 end.
 
 Definition fv_redlabel (rl5:redlabel) : list value_name :=
@@ -242,26 +157,29 @@ Inductive VTSin : value_name -> typexpr -> G -> Prop :=    (* defn VTSin *)
      VTSin value_name5 typexpr5 G5 ->
       not(  value_name5 = value_name'  )  ->
      VTSin value_name5 typexpr5 (G_vn G5 value_name' typexpr')
-with G_constant : G -> constant -> typexpr -> Prop :=    (* defn G_constant *)
- | constant_ret : forall (G5:G) (t:typexpr),
-     G_constant G5 CONST_ret (TE_arrow t (TE_concurrent t))
- | constant_fork : forall (G5:G) (t1 t2:typexpr),
-     G_constant G5 CONST_fork (TE_arrow  (TE_concurrent t1)   (TE_arrow  (TE_concurrent t2)   (TE_concurrent  (TE_sum  (TE_prod t1  (TE_concurrent t2) )   (TE_prod  (TE_concurrent t1)  t2) ) ) ) )
- | constant_unit : forall (G5:G),
-     G_constant G5 CONST_unit (TE_constants TC_unit)
- | constant_pair : forall (G5:G) (t1 t2:typexpr),
-     G_constant G5 CONST_pair (TE_arrow t1  (TE_arrow t2  (TE_prod t1 t2) ) )
- | constant_proj1 : forall (G5:G) (t1 t2:typexpr),
-     G_constant G5 CONST_proj1 (TE_arrow  (TE_prod t1 t2)  t1)
- | constant_proj2 : forall (G5:G) (t1 t2:typexpr),
-     G_constant G5 CONST_proj2 (TE_arrow  (TE_prod t1 t2)  t2)
 with Get : G -> expr -> typexpr -> Prop :=    (* defn Get *)
+ | Get_ret : forall (G5:G) (e:expr) (t:typexpr),
+     Get G5 e t ->
+     Get G5 (E_ret e) (TE_concurrent t)
+ | Get_fork : forall (G5:G) (e e':expr) (t1 t2:typexpr),
+     Get G5 e  (TE_concurrent t1)  ->
+     Get G5 e'  (TE_concurrent t2)  ->
+     Get G5 (E_fork e e')  (TE_concurrent  (TE_sum  (TE_prod t1  (TE_concurrent t2) )   (TE_prod  (TE_concurrent t1)  t2) ) ) 
+ | Get_unit : forall (G5:G),
+     Get G5 E_unit TE_unit
+ | Get_inpair : forall (G5:G) (e e':expr) (t1 t2:typexpr),
+     Get G5 e t1 ->
+     Get G5 e' t2 ->
+     Get G5 (E_inpair e e')  (TE_prod t1 t2) 
+ | Get_proj1 : forall (G5:G) (e:expr) (t1 t2:typexpr),
+     Get G5 e  (TE_prod t1 t2)  ->
+     Get G5 (E_proj1 e) (TE_arrow  (TE_prod t1 t2)  t1)
+ | Get_proj2 : forall (G5:G) (e:expr) (t1 t2:typexpr),
+     Get G5 e  (TE_prod t1 t2)  ->
+     Get G5 (E_proj2 e) (TE_arrow  (TE_prod t1 t2)  t2)
  | Get_value_name : forall (G5:G) (x:value_name) (t:typexpr),
      VTSin x t G5 ->
      Get G5 (E_ident x) t
- | Get_constant : forall (G5:G) (constant5:constant) (t:typexpr),
-     G_constant G5 constant5 t ->
-     Get G5 (E_constant constant5) t
  | Get_apply : forall (G5:G) (e e':expr) (t2 t1:typexpr),
      Get G5 e (TE_arrow t1 t2) ->
      Get G5 e' t1 ->
@@ -306,23 +224,33 @@ Inductive JO_red : expr -> select -> redlabel -> expr -> Prop :=    (* defn red 
      JO_red (E_apply  (E_function x t e)  v) s RL_tau  (subst_expr  v   x   e ) 
  | JO_red_docomp : forall (e:expr) (s:select),
      JO_red (E_comp e) s (RL_labelled e) e
+ | JO_red_forkeval1 : forall (e e':expr) (s:select) (rl:redlabel) (e'':expr),
+     JO_red e s rl e'' ->
+     JO_red (E_fork e e') s rl (E_fork e'' e')
+ | JO_red_forkeval2 : forall (v e':expr) (s:select) (rl:redlabel) (e'':expr),
+     is_value_of_expr v ->
+     JO_red e' s rl e'' ->
+     JO_red (E_fork v e') s rl (E_fork v e'')
  | JO_red_forkmove1 : forall (e e':expr) (rl:redlabel) (e'':expr) (s:select),
      JO_red e s rl e'' ->
      ~ (is_value_of_expr e')  ->
-     JO_red (E_apply  (E_apply (E_constant CONST_fork)  (E_live_expr e) )   (E_live_expr e') ) S_First rl (E_apply  (E_apply (E_constant CONST_fork)  (E_live_expr e'') )   (E_live_expr e') )
+     JO_red (E_fork  (E_live_expr e)   (E_live_expr e') ) S_First rl (E_fork  (E_live_expr e'')   (E_live_expr e') )
  | JO_red_forkmove2 : forall (e e':expr) (rl:redlabel) (e'':expr) (s:select),
      JO_red e' s rl e'' ->
      ~ (is_value_of_expr e)  ->
-     JO_red (E_apply  (E_apply (E_constant CONST_fork)  (E_live_expr e) )   (E_live_expr e') ) S_Second rl (E_apply  (E_apply (E_constant CONST_fork)  (E_live_expr e) )   (E_live_expr e'') )
+     JO_red (E_fork  (E_live_expr e)   (E_live_expr e') ) S_Second rl (E_fork  (E_live_expr e)   (E_live_expr e'') )
  | JO_red_forkdeath1 : forall (v e:expr),
      is_value_of_expr v ->
-     JO_red (E_apply  (E_apply (E_constant CONST_fork)  (E_live_expr v) )   (E_live_expr e) ) S_First RL_tau (E_live_expr  (E_taggingleft   (E_pair v  (E_live_expr e) )  ) )
+     JO_red (E_fork  (E_live_expr v)   (E_live_expr e) ) S_First RL_tau (E_live_expr  (E_taggingleft   (E_pair v  (E_live_expr e) )  ) )
  | JO_red_forkdeath2 : forall (e v':expr),
      is_value_of_expr v' ->
-     JO_red (E_apply  (E_apply (E_constant CONST_fork)  (E_live_expr e) )   (E_live_expr v') ) S_Second RL_tau (E_live_expr  (E_taggingright  (E_pair  (E_live_expr e)  v') ) )
+     JO_red (E_fork  (E_live_expr e)   (E_live_expr v') ) S_Second RL_tau (E_live_expr  (E_taggingright  (E_pair  (E_live_expr e)  v') ) )
  | JO_red_ret : forall (v:expr) (s:select),
      is_value_of_expr v ->
-     JO_red (E_apply (E_constant CONST_ret) v) s RL_tau  (E_live_expr v) 
+     JO_red (E_ret v) s RL_tau  (E_live_expr v) 
+ | JO_red_evalret : forall (e:expr) (s:select) (rl:redlabel) (e':expr),
+     JO_red e s rl e' ->
+     JO_red (E_ret e) s rl (E_ret e')
  | JO_red_evalbind : forall (e e'':expr) (s:select) (rl:redlabel) (e':expr),
      JO_red e s rl e' ->
      JO_red (E_bind e e'') s rl (E_bind e' e'')
@@ -354,15 +282,28 @@ Inductive JO_red : expr -> select -> redlabel -> expr -> Prop :=    (* defn red 
  | JO_red_inpair : forall (v v':expr) (s:select),
      is_value_of_expr v ->
      is_value_of_expr v' ->
-     JO_red (E_apply  (E_apply (E_constant CONST_pair) v)  v') s RL_tau (E_pair v v')
+     JO_red (E_inpair v v') s RL_tau (E_pair v v')
+ | JO_red_inpair_eval1 : forall (e e':expr) (s:select) (rl:redlabel) (e'':expr),
+     JO_red e s rl e'' ->
+     JO_red (E_inpair e e') s rl (E_inpair e'' e')
+ | JO_red_inpair_eval2 : forall (v e':expr) (s:select) (rl:redlabel) (e'':expr),
+     is_value_of_expr v ->
+     JO_red e' s rl e'' ->
+     JO_red (E_inpair v e') s rl (E_inpair v e'')
  | JO_red_proj1 : forall (v v':expr) (s:select),
      is_value_of_expr v ->
      is_value_of_expr v' ->
-     JO_red (E_apply (E_constant CONST_proj1) (E_pair v v')) s RL_tau v
+     JO_red (E_proj1 (E_pair v v')) s RL_tau v
  | JO_red_proj2 : forall (v v':expr) (s:select),
      is_value_of_expr v ->
      is_value_of_expr v' ->
-     JO_red (E_apply (E_constant CONST_proj2) (E_pair v v')) s RL_tau v'
+     JO_red (E_proj2 (E_pair v v')) s RL_tau v'
+ | JO_red_proj1_eval : forall (e:expr) (s:select) (rl:redlabel) (e':expr),
+     JO_red e s rl e' ->
+     JO_red (E_proj1 e) s rl (E_proj1 e')
+ | JO_red_proj2_eval : forall (e:expr) (s:select) (rl:redlabel) (e':expr),
+     JO_red e s rl e' ->
+     JO_red (E_proj2 e) s rl (E_proj2 e')
  | JO_red_evalinl : forall (e:expr) (s:select) (rl:redlabel) (e':expr),
      JO_red e s rl e' ->
      JO_red (E_taggingleft e) s rl (E_taggingleft e')
