mconbaseMonProofs.v
@@ -7,7 +7,7 @@ Load redTotalDetProp.
 
 Lemma mon_left_id : forall (x:value_name) (t : typexpr) (a e:expr) (s s' : select),
     is_value_of_expr a ->
-    ((E_apply(E_constant (CONST_ret)) a) >>= (E_function x t e)) -->* (E_apply (E_function x t e) a).
+    ((E_ret a) >>= (E_function x t e)) -->* (E_apply (E_function x t e) a).
 Proof.
  intros.
  apply JO_red_star_step with (e' := (E_live_expr ( a) >>= E_function x t e))(s:=s)(rl:=RL_tau).
@@ -20,204 +20,418 @@ Proof.
  apply JO_red_star_refl.
 Qed.
 
-Lemma mon_left_id_wbsm : forall (x:value_name) (t : typexpr) (a e:expr),
-    is_value_of_expr a ->
-    weakbisim ((E_apply(E_constant (CONST_ret)) a) >>= (E_function x t e)) (E_apply (E_function x t e) a).
+
+Inductive mon_left_id_rel : relation expr :=
+| mon_left_id_bound : forall (e e' : expr), is_value_of_expr e' -> mon_left_id_rel ((E_ret e) >>= e') (E_apply e' e)
+| mon_left_id_inbound : forall (e e' : expr), is_value_of_expr e' -> mon_left_id_rel ((E_live_expr e) >>= e') (E_apply e' e)
+| mon_left_id_unbound : forall (e : expr), mon_left_id_rel (e) (e).
+
+
+Theorem mon_left_id_wbsm : isExprRelationStepWeakBisimilarity mon_left_id_rel.
 Proof.
- intros.
- cut (totalTauRed ((E_apply(E_constant (CONST_ret)) a) >>= (E_function x t e)) (E_apply (E_function x t e) a)).
- intros.
- apply bisimsymm.
- apply ttau_weakbisim_incl.
- trivial.
- intros.
- apply S_star with (y:=((E_live_expr ( a) >>= E_function x t e))).
- apply JO_red_evalbind_td.
- apply JO_red_ret_td.
- apply S_First.
- trivial.
- intros.
+ unfold isExprRelationStepWeakBisimilarity.
+ intuition.
+ inversion H.
+ substs.
+ inversion H0.
+ substs.
+ inversion H7.
+ substs.
+ exists (E_apply e' e).
+ Hint Constructors mon_left_id_rel.
+ intuition.
+ apply weakred_T.
+ apply star_refl.
+ substs.
+ exists (E_apply e' e'1).
+ intuition.
+ induction rl.
+ apply weakred_T.
+ apply star1.
+ apply tStep with (s:=s).
+ apply JO_red_context_app2.
+ assumption.
+ assumption.
+ apply weakred_L.
+ apply lab_r with (e1:=(E_apply e' e))(e2:=(E_apply e' e'1))(s:=s).
+ splits.
+ apply star_refl.
+ apply JO_red_context_app2; auto.
+ apply star_refl.
+ substs.
+ inversion H0.
+ apply red_not_value in H7; simpl in H7; intuition.
+ substs.
+ exists ((E_apply e' e'0)).
+ intuition.
+ induction rl.
+ apply weakred_T.
+ apply star1.
+ apply tStep with (s:=s).
+ apply JO_red_context_app2.
+ assumption.
+ assumption.
+ apply weakred_L.
+ apply lab_r with (e1:=(E_apply e' e))(e2:=(E_apply e' e'0))(s:=s).
+ intuition.
+ apply star_refl.
+ apply JO_red_context_app2.
+ assumption.
+ assumption.
+ apply star_refl.
+ substs.
+ exists ((E_apply e' e) ).
+ Hint Constructors weakred.
+ intuition.
+ apply weakred_T.
+ apply star_refl.
+ substs.
+ exists p'.
+ intuition.
+ induction rl.
+ apply weakred_T.
+ apply star1.
+ apply simpTau in H0.
+ assumption.
+ apply weakred_L.
+ apply lab_r with (e1:=q)(e2:=p')(s:=s).
+ intuition.
+ apply star_refl.
+ apply star_refl.
+ inversion H.
+ substs.
+ inversion H0.
+ substs.
+ exists (subst_expr e x e0).
+ intuition.
+ apply weakred_T.
+ apply S_star with (y:=((E_live_expr e)) >>= E_function x t e0).
+ apply tStep with (s:=S_First).
  apply JO_red_evalbind.
  apply JO_red_ret.
- trivial.
- apply S_star with (y:=(E_apply (E_function x t e) a)).
- apply JO_red_dobind_td.
- apply S_First.
- trivial.
+ assumption.
+ apply S_star with (y:=(E_apply (E_function x t e0) e)).
+ apply tStep with (s:=S_First).
+ apply JO_red_dobind.
+ assumption.
+ apply star1.
+ apply tStep with (s:=S_First).
+ apply JO_red_app.
+ assumption.
+ substs.
+ exists (E_ret e'' >>= e').
+ intuition.
+ induction rl.
+ apply weakred_T.
+ apply star1.
+ apply tStep with (s:=s).
+ apply JO_red_evalbind.
+ apply JO_red_evalret.
+ assumption.
+ apply weakred_L.
+ apply lab_r with (e1:=(E_ret e >>= e') )(e2:=(E_ret e'' >>= e'))(s:=s); intuition.
+ apply star_refl.
+ apply JO_red_evalbind.
+ apply JO_red_evalret.
+ assumption.
+ apply star_refl.
+ substs.
+ apply red_not_value in H7; contradiction.
+ substs.
+ inversion H0.
+ substs.
+ exists (subst_expr e x e0).
+ intuition.
+ apply weakred_T.
+ apply S_star with (y:=(E_apply (E_function x t e0) e)).
+ apply tStep with (s:=S_First).
+ apply JO_red_dobind.
+ assumption.
+ apply star1.
+ apply tStep with (s:=S_First).
+ apply JO_red_app.
+ assumption.
+ substs.
+ exists ((E_live_expr e'' >>= e')); intuition.
+ induction rl.
+ apply weakred_T.
+ apply star1.
+ apply tStep with (s:=s).
+ apply JO_red_movebind.
+ assumption.
+ apply weakred_L.
+ apply lab_r with (e1:=(E_live_expr e >>= e'))(e2:=(E_live_expr e'' >>= e'))(s:=s).
+ splits.
+ apply star_refl.
+ apply JO_red_movebind.
+ assumption.
+ apply star_refl.
+ substs.
+ apply red_not_value in H7; contradiction.
+ substs.
+ exists q'.
+ intuition.
+ induction rl.
+ apply weakred_T.
+ apply star1.
+ apply tStep in H0; assumption.
+ apply weakred_L.
+ apply lab_r with (e1:=q)(e2:=q')(s:=s).
+ splits.
+ apply star_refl.
+ assumption.
  apply star_refl.
 Qed.
+ 
+Inductive mon_right_id_rel : relation expr :=
+| mon_right_id_bound : forall (a : expr) (x : value_name) (t : typexpr), is_value_of_expr a -> mon_right_id_rel (E_live_expr (a) >>= (E_function x t (E_ret (E_ident x))))  (E_live_expr ( a))
+| mon_right_id_inbound : forall (a : expr) (x : value_name) (t : typexpr), is_value_of_expr a -> mon_right_id_rel (E_apply (E_function x t (E_ret (E_ident x))) ( (a)))  (E_live_expr ( a))
+| mon_right_id_unbound : forall (a : expr), is_value_of_expr a -> mon_right_id_rel ( ( (E_ret (a))) )  (E_live_expr ( a))
+| mon_right_id_ret : forall (a : expr), mon_right_id_rel (E_live_expr ( a))  (E_live_expr ( a)).
 
 
-Lemma mon_right_id : forall (a:expr) (s s' : select),
-   is_value_of_expr a ->
-   E_live_expr (a) >>= E_constant CONST_ret -->* E_live_expr ( a).
+Theorem mon_right_id_wbsm : isExprRelationStepWeakBisimilarity mon_right_id_rel.
 Proof.
+ unfold isExprRelationStepWeakBisimilarity.
  intros.
- apply JO_red_star_step with (e' := (E_apply (E_constant CONST_ret) a))(s:= s)(rl:=RL_tau).
- apply JO_red_dobind.
- trivial.
- apply JO_red_star_step with (e' := (E_live_expr (a)))(s:=s')(rl:=RL_tau).
- apply JO_red_ret.
- trivial.
- apply JO_red_star_refl.
-Qed.
-
-Lemma mon_right_id_wbsm : forall (a:expr) (s s' : select),
-   is_value_of_expr a ->
-   weakbisim (E_live_expr (a) >>= E_constant CONST_ret) (E_live_expr (a)).
-Proof.
-  intros.
-  cut (totalTauRed (E_live_expr (a) >>= E_constant CONST_ret) (E_live_expr (a))).
-  intros.
-  apply bisimsymm.
-  apply ttau_weakbisim_incl.
-  trivial.
-  apply S_star with (y:=(E_apply (E_constant CONST_ret) a)).
-  apply JO_red_dobind_td.
-  trivial.
-  trivial.
-  apply S_star with (y:=(E_live_expr ( a))).
-  apply JO_red_ret_td.
-  trivial. trivial.
-  apply star_refl.
-Qed.
-
-Lemma mon_assoc : forall (v v' v'' : value_name) (t t' : typexpr) (a e e' :expr)(s s' s'':select),  
-    is_value_of_expr a ->
-    v <> v'' ->
-    v' <> v'' ->
-    ((subst_expr a v'' e') = e') ->
-    ((subst_expr a v'' e) = e) ->
-    exists (b :expr), (E_live_expr (a) >>= (E_function v t e) >>= (E_function v' t' e') -->* b) /\ (E_live_expr (a) >>= (E_function v'' t (E_apply (E_function v t e) (E_ident v'') >>= (E_function v' t' e'))) -->* b).
-Proof.
+ inversion H.
+ substs.
+ splits.
  intros.
- exists (E_apply (E_function v t e) a >>= E_function v' t' e' ).
- split.
- Show 1.
-  apply JO_red_star_step with (e' := ((E_apply (E_function v t e) a) >>= E_function v' t' e'))(s:=s)(rl:=RL_tau).
-  apply JO_red_evalbind with (e' := ((E_apply (E_function v t e) a))).
-  apply JO_red_dobind.
-  trivial.
-  apply JO_red_star_refl.
- apply JO_red_star_step with (e' := (E_apply (E_function v'' t (E_apply (E_function v t e) (E_ident v'') >>= E_function v' t' e')) a))(s:=s')(rl:=RL_tau).
- apply JO_red_dobind.
- trivial.
- apply JO_red_star_step with  (e' := (subst_expr a v'' (E_apply (E_function v t e) (E_ident v'') >>= E_function v' t' e')))(s:=s'')(rl:=RL_tau).
- apply JO_red_app with (x:=v'') (v:=a) (e := (E_apply (E_function v t e) (E_ident v'') >>= E_function v' t' e')).
- trivial.
- auto.
- cut ((subst_expr a v''  (E_apply (E_function v t e) (E_ident v'') >>= E_function v' t' e') = (E_apply (E_function v t e) a >>= E_function v' t' e'))). 
- intros.
- rewrite H4.
- apply JO_red_star_refl.
- simpl.
- rewrite H2.
- rewrite H3.
- cut ((if eq_value_name v v'' then true else false) = false).
- intros.
- rewrite H4.
- cut ((if eq_value_name v'' v'' then a else E_ident v'') = a).
- intros.
- rewrite H5.
- cut ((if eq_value_name v' v'' then true else false) = false).
- intros.
- rewrite H6.
- trivial.
- Check eq_value_name v v''.
- destruct (eq_value_name v v'').
- contradiction.
- destruct (eq_value_name v' v'').
- contradiction.
- trivial.
- destruct (eq_value_name v'' v'').
- trivial.
- contradiction n.
- trivial.
- destruct (eq_value_name v v'').
- contradiction e0.
- trivial.
-Qed.
-
-
-
-Lemma mon_assoc_wbsm : forall (v v' v'' : value_name) (t t' : typexpr) (a e e' :expr)(s s' s'':select),  
-    is_value_of_expr a ->
-    v <> v'' ->
-    v' <> v'' ->
-    ((subst_expr a v'' e') = e') ->
-    ((subst_expr a v'' e) = e) ->
-    weakbisim (E_live_expr (a) >>= (E_function v t e) >>= (E_function v' t' e')) (E_live_expr (a) >>= (E_function v'' t (E_apply (E_function v t e) (E_ident v'') >>= (E_function v' t' e')))).
-Proof.
- intros.
- cut (exists (b :expr), (weakbisim (E_live_expr (a) >>= (E_function v t e) >>= (E_function v' t' e')) b) /\ (weakbisim (E_live_expr (a) >>= (E_function v'' t (E_apply (E_function v t e) (E_ident v'') >>= (E_function v' t' e')))) b)).
- intros.
- elim H4.
- intros.
- elim H5; intros.
- apply bisimsymm in H7.
- apply bisimtrans with (e':=x).
- auto.
- intros.
- exists (E_apply (E_function v t e) a >>= E_function v' t' e' ).
- split.
- Show 1.
-  cut (totalTauRed (E_live_expr (a) >>= E_function v t e >>= E_function v' t' e') (E_apply (E_function v t e) a >>= E_function v' t' e')).
-  intros.
-  apply bisimsymm.
-  apply ttau_weakbisim_incl.
-  trivial.
-  apply S_star with (y := ((E_apply (E_function v t e) a) >>= E_function v' t' e')).
-  apply JO_red_evalbind_td.
-  apply JO_red_dobind_td.
-  trivial.
-  trivial.
-  intros.
-  apply JO_red_evalbind.
-  apply JO_red_dobind.
-  trivial.
-  apply star_refl.
- Show 1.
- cut (totalTauRed (E_live_expr (a) >>=   E_function v'' t (E_apply (E_function v t e) (E_ident v'') >>= E_function v' t' e')) (E_apply (E_function v t e) a >>= E_function v' t' e')).
- intros.
- apply bisimsymm.
- apply ttau_weakbisim_incl.
- trivial.
- apply S_star with (y := (E_apply (E_function v'' t (E_apply (E_function v t e) (E_ident v'') >>= E_function v' t' e')) a)).
- apply JO_red_dobind_td.
- trivial.
- trivial.
- apply S_star with  (y := (subst_expr a v'' (E_apply (E_function v t e) (E_ident v'') >>= E_function v' t' e'))).
- apply JO_red_app_td.
- trivial.
- cut ((subst_expr a v''  (E_apply (E_function v t e) (E_ident v'') >>= E_function v' t' e') = (E_apply (E_function v t e) a >>= E_function v' t' e'))). 
- intros.
- rewrite H4.
+ exists (E_live_expr a).
+ inversion H1.
+ apply red_not_value in H7; simpl in H7; intuition.
+ apply red_not_value in H7; simpl in H7; intuition.
+ substs.
+ Hint Constructors mon_right_id_rel.
+ intuition.
+ apply weakred_T.
  apply star_refl.
+ intros.
+ apply red_not_value in H1; simpl in H1; intuition.
+ substs.
+ splits.
+ intros.
+ exists (E_live_expr a).
+ inversion H1.
+ substs.
  simpl.
- rewrite H2.
- rewrite H3.
- cut ((if eq_value_name v v'' then true else false) = false).
+ destruct (eq_value_name x x).
+ intuition.
+ apply weakred_T.
+ apply star_refl.
+ intuition.
+ substs.
+ apply red_not_value in H8; simpl in H8; intuition.
+ substs.
+ apply red_not_value in H7; simpl in H7; intuition.
  intros.
- rewrite H4.
- cut ((if eq_value_name v'' v'' then a else E_ident v'') = a).
+ apply red_not_value in H1; simpl in H1; intuition.
+ substs.
+ splits.
  intros.
- rewrite H5.
- cut ((if eq_value_name v' v'' then true else false) = false).
+ exists (E_live_expr a).
+ inversion H1.
+ substs.
+ splits.
+ apply weakred_T.
+ apply star_refl.
+ auto.
+ substs.
+ apply red_not_value in H3; simpl in H3; intuition.
  intros.
- rewrite H6.
- trivial.
- Check eq_value_name v v''.
- destruct (eq_value_name v v'').
- contradiction.
- destruct (eq_value_name v' v'').
- contradiction.
- trivial.
- destruct (eq_value_name v'' v'').
- trivial.
- contradiction n.
- trivial.
- destruct (eq_value_name v v'').
- contradiction e0.
- trivial.
+ apply red_not_value in H1; simpl in H1; intuition.
+ substs.
+ splits.
+ intros.
+ apply red_not_value in H0; simpl in H0; intuition.
+ intros.
+ apply red_not_value in H0; simpl in H0; intuition.
 Qed.
 
+Definition exprClosedOnVariable : expr -> value_name -> Prop := fun e v => 
+     ( forall (e' : expr), (subst_expr e' v e) = e ).
+
+Inductive mon_assoc_rel : relation expr :=
+| mon_assoc_start : forall (e e' e'' : expr) (v v' v'' : value_name) (t t' : typexpr), v <> v'' -> v' <> v'' -> exprClosedOnVariable e' v'' -> exprClosedOnVariable e'' v'' ->
+    mon_assoc_rel (e >>= (E_function v t e') >>= (E_function v' t' e'')) (e >>= (E_function v'' t (E_apply (E_function v t e') (E_ident v'') >>= (E_function v' t' e''))))
+| mon_assoc_s1 : forall (e e' e'' : expr) (v v' v'' : value_name) (t t' : typexpr), v <> v'' -> v' <> v'' -> is_value_of_expr e ->  exprClosedOnVariable e' v'' -> exprClosedOnVariable e'' v'' ->
+    mon_assoc_rel ( (E_apply (E_function v t e') e ) >>= (E_function v' t' e'')) (E_apply (E_function v'' t (E_apply (E_function v t e') (E_ident v'') >>= (E_function v' t' e''))) e)
+| mon_assoc_s2 : forall (e e' e'' : expr) (v v' v'' : value_name) (t t' : typexpr), v <> v'' -> v' <> v'' -> is_value_of_expr e -> exprClosedOnVariable e' v'' -> exprClosedOnVariable e'' v'' ->
+    mon_assoc_rel ( ( ( (subst_expr e v e'))  ) >>= (E_function v' t' e''))    ( ( ((E_apply (E_function v t e') e) >>= (E_function v' t' e''))) )
+| mon_assoc_s3 : forall (e e' e'' : expr) (v v' : value_name) (t t' : typexpr), is_value_of_expr e -> 
+    mon_assoc_rel ( ( ( (subst_expr e v e'))  ) >>= (E_function v' t' e''))    ( ( ((subst_expr e v e') >>= (E_function v' t' e''))) )
+| mon_assoc_fin : forall (e : expr) , 
+    mon_assoc_rel e e.
+
+Hint Constructors mon_assoc_rel.
+
+Theorem mon_assoc_wbsm: isExprRelationStepWeakBisimilarity mon_assoc_rel.
+Proof.
+ unfold isExprRelationStepWeakBisimilarity.
+ intros.
+ inversion H.
+ substs.
+ splits.
+ intros.
+ inversion H4.
+ substs.
+ inversion H10.
+ substs.
+ Hint Unfold exprClosedOnVariable.
+ exists ((e'1 >>=
+       E_function v'' t
+         (E_apply (E_function v t e') (E_ident v'') >>= E_function v' t' e''))).
+ intuition.
+ apply simpl_weakred with (s:=s).
+ apply JO_red_evalbind.
+ assumption.
+ substs.
+ exists ((E_live_expr e'1 >>=
+       E_function v'' t
+         (E_apply (E_function v t e') (E_ident v'') >>= E_function v' t' e''))).
+ intuition.
+ apply simpl_weakred with (s:=s).
+ apply JO_red_movebind.
+ assumption.
+ substs. 
+ exists ((E_apply (E_function v'' t (E_apply (E_function v t e') (E_ident v'') >>= (E_function v' t' e''))) v0)).
+ intuition.
+ apply simpl_weakred with (s:=s).
+ apply JO_red_dobind.
+ assumption.
+ intros.
+ inversion H4.
+ substs.
+ exists (e'0 >>= E_function v t e' >>= E_function v' t' e'').
+ intuition.
+ apply simpl_weakred with (s:=s).
+ apply JO_red_evalbind.
+ apply JO_red_evalbind.
+ assumption.
+ substs.
+ exists (E_live_expr e'0 >>= E_function v t e' >>= E_function v' t' e'').
+ intuition.
+ apply simpl_weakred with (s:=s).
+ apply JO_red_evalbind.
+ apply JO_red_movebind.
+ assumption.
+ substs.
+ exists ( (E_apply (E_function v t e') v0 ) >>= (E_function v' t' e'')).
+ intuition.
+ apply simpl_weakred with (s:=s).
+ apply JO_red_evalbind.
+ apply JO_red_dobind.
+ assumption.
+ intros.
+ 
+ splits.
+ intros.
+ substs.
+ inversion H7.
+ substs.
+ inversion H11.
+ substs.
+ exists ( ( ((E_apply (E_function v t e') e) >>= (E_function v' t' e''))) ).
+ intuition.
+ apply simpl_weakred with (s:=s).
+ assert ((subst_expr e v'' (E_apply (E_function v t e') (E_ident v'') >>= E_function v' t' e'')) = E_apply (E_function v t e') e >>= E_function v' t' e'').
+ simpl.
+ assert (subst_expr e v'' e' = e'); intuition.
+  assert (subst_expr e v'' e'' = e''); intuition.
+ rewrite -> H5; rewrite -> H6.
+ destruct (eq_value_name v v''); destruct (eq_value_name v'' v''); destruct (eq_value_name v' v''); intuition.
+ rewrite <- H5.
+ apply JO_red_app.
+ assumption.
+ intuition.
+ apply mon_assoc_s2 with (v'':=v''); intuition.
+ substs.
+ apply red_not_value in H13; simpl in H13; intuition.
+ apply red_not_value in H12; simpl in H12; intuition.
+ intros.
+ substs.
+ inversion H7.
+ substs.
+ simpl in H7.
+ simpl.
+ assert (subst_expr e v'' e' = e'); intuition.
+ assert (subst_expr e v'' e'' = e''); intuition.
+ destruct (eq_value_name v v''); destruct (eq_value_name v'' v''); destruct (eq_value_name v' v''); intuition.
+ rewrite -> H5 in H7; rewrite -> H6 in H7.
+ rewrite -> H5; rewrite -> H6.
+ exists (E_apply (E_function v t e') e >>= E_function v' t' e'').
+ intuition.
+ apply weakred_T.
+ apply star_refl.
+ substs.
+ apply red_not_value in H12; simpl in H12; intuition.
+ substs.
+ apply red_not_value in H11; simpl in H11; intuition.
+ substs.
+ splits.
+ intros.
+ inversion H5.
+ substs.
+ exists (e'0 >>= E_function v' t' e'').
+ intuition.
+ apply weakred_tau_prefix with (e':=(subst_expr e v e' >>= E_function v' t' e'')).
+ apply simpl_weakred with (s:=S_First).
+ apply JO_red_evalbind.
+ apply JO_red_app.
+ assumption.
+ apply simpl_weakred with (s:=s).
+ apply JO_red_evalbind.
+ assumption.
+ substs.
+ exists (E_live_expr e'0 >>= E_function v' t' e'').
+ intuition.
+ apply weakred_tau_prefix with (e':=(subst_expr e v e' >>= E_function v' t' e'')).
+ apply simpl_weakred with (s:=S_First).
+ apply JO_red_evalbind.
+ apply JO_red_app.
+ assumption.
+ rewrite <- H6.
+ apply simpl_weakred with (s:=s).
+ apply JO_red_movebind.
+ assumption.
+ substs.
+ exists (E_apply (E_function v' t' e'') v0).
+ intuition.
+ apply weakred_tau_prefix with (e':=(subst_expr e v e' >>= E_function v' t' e'')).
+ apply simpl_weakred with (s:=S_First).
+ apply JO_red_evalbind.
+ apply JO_red_app.
+ assumption.
+ rewrite <- H6.
+ apply simpl_weakred with (s:=S_First).
+ apply JO_red_dobind.
+ assumption.
+ intros.
+ inversion H5.
+ substs.
+ inversion H11.
+ substs.
+ exists (subst_expr e v e' >>= E_function v' t' e'').
+ intuition.
+ apply weakred_T.
+ apply star_refl.
+ apply red_not_value in H13; simpl in H13; intuition.
+ apply red_not_value in H12; simpl in H12; intuition.
+ substs.
+ split.
+ intros.
+ exists p'.
+ split; [eauto | auto ].
+ intros.
+ exists q'.
+ split; [eauto | auto ].
+ substs.
+ split.
+ intros.
+ exists p'.
+ split; [eauto | auto ].
+ intros.
+ exists q'.
+ split; [eauto | auto ].
+Qed.
