mconextract.v
@@ -16,37 +16,24 @@ Load progress.
 Fixpoint xis_value_of_expr (e_5:expr) : bool :=
   match e_5 with
   | (E_ident value_name5) => false
-  | (E_constant constant5) => (true)
-  | (E_apply (E_constant (CONST_fork)) e) => ((xis_value_of_expr e))
-  | (E_apply (E_constant (CONST_pair)) e) => ((xis_value_of_expr e))
-  | (E_apply expr5 expr') => match expr5 with | E_constant (CONST_fork) => xis_value_of_expr (expr') | E_constant (CONST_pair) => xis_value_of_expr (expr') | _ => false end  
+  | E_unit => (true)
+  | (E_apply expr5 expr') => false
   | (E_bind expr5 expr') => false
-  | (E_function value_name5 typexpr5 expr5) => true
+  | (E_function value_name5 typexpr5 expr5) => (true)
   | (E_fix e) => false
-  | (E_comp lab) => false
-  | (E_live_expr expr5) => true
+  | (E_comp e) => false
+  | (E_live_expr e) => (true)
   | (E_pair e e') => (if (xis_value_of_expr e) then (xis_value_of_expr e') else false)
+  | (E_inpair e e') => false
+  | (E_proj1 e) => false
+  | (E_proj2 e) => false
+  | (E_fork e e') => false
+  | (E_ret e) => false
   | (E_taggingleft e) => ((xis_value_of_expr e))
   | (E_taggingright e) => ((xis_value_of_expr e))
   | (E_case e1 x1 e2 x2 e3) => false
 end.
 
-(*
-Fixpoint xis_forkvalue (e : expr) : bool :=
-  match e with
-  | (E_ident value_name5) => false
-  | (E_constant constant5) => match constant5 with | CONST_fork => false | CONST_ret => true | CONST_unit => false | CONST_stop => true end
-  | (E_apply (E_constant (CONST_fork)) e) => ((xis_value_of_expr e))
-  | (E_apply expr5 expr') => false
-  | (E_bind expr5 expr') => false
-  | (E_function value_name5 typexpr5 expr5) => false
-  | (E_fix e) => (xis_value_of_expr e)
-  | (E_live_expr lm) => match lm with |  => false |  e' => (xis_value_of_expr e') end
-  | (E_pair e e') => false
-  | (E_taggingleft e) => false
-  | (E_taggingright e) => false
-  | (E_case e1 x1 e2 x2 e3) => false
-end. *)
 
 (* Proof that is_value_of_expr and xis_value_of_expr are equivalent *)
 
@@ -56,12 +43,17 @@ Recursive Extraction selectstar.
 
 (* Extractable version of the reduction operation *)
 Inductive XJO_red : expr -> selectstar -> expr -> Prop :=    (* defn red *)
-(* | XJO_red_app : forall (x:value_name) (t : typexpr) (e v:expr) (s:selectstar),
+(* 
+ | XJO_red_app : forall (x:value_name) (t : typexpr) (e v:expr) (s:selectstar),
      (eq (xis_value_of_expr v) true) ->
      XJO_red (E_apply  (E_function x t e)  v) s  (subst_expr  v   x   e ) 
  | XJO_red_ret : forall (v:expr) (s:selectstar),
      (eq (xis_value_of_expr v) true) ->
-     XJO_red (E_apply (E_constant CONST_ret) v) s (E_live_expr ( (v))) 
+     XJO_red (E_ret v) s (E_live_expr ( (v))) 
+ | XJO_red_evalret : forall (v v':expr) (s:selectstar),
+     (eq (xis_value_of_expr v) false) ->
+     XJO_red v s v' ->
+     XJO_red (E_ret v) s  (E_ret v') 
  | XJO_red_evalbind : forall (e e'' e':expr) (s:selectstar),
     (eq (xis_value_of_expr e) false) ->
      XJO_red e s e' ->
@@ -76,33 +68,60 @@ Inductive XJO_red : expr -> selectstar -> expr -> Prop :=    (* defn red *)
  | XJO_red_inpair : forall (v v':expr) (s:selectstar),
      (eq (xis_value_of_expr v) true) ->
      (eq (xis_value_of_expr v') true) ->
-     XJO_red (E_apply  (E_apply (E_constant CONST_pair) v)  v') s (E_pair v v') 
+     XJO_red (E_inpair v  v') s (E_pair v v')
+ | XJO_red_inpair_eval2 : forall (v v' v'' :expr) (s:selectstar),
+     (eq (xis_value_of_expr v) true) ->
+     (eq (xis_value_of_expr v') false) ->
+     XJO_red v' s v'' ->
+     XJO_red (E_inpair v  v') s (E_inpair v v'')  
+ | XJO_red_inpair_eval1 : forall (v v' v'' :expr) (s:selectstar),
+     (eq (xis_value_of_expr v) false) ->
+     XJO_red v s v'' ->
+     XJO_red (E_inpair v  v') s (E_inpair v'' v') 
  | XJO_red_docomp : forall (e:expr) (s:selectstar),
      XJO_red (E_comp e) s e
  | XJO_red_proj1 : forall (v v':expr) (s:selectstar),
      (eq (xis_value_of_expr v) true) ->
      (eq (xis_value_of_expr v') true) ->
-     XJO_red (E_apply (E_constant CONST_proj1) (E_pair v v')) s v
+     XJO_red (E_proj1 (E_pair v v')) s v
+ | XJO_red_proj1_eval : forall (v v':expr) (s:selectstar),
+     (eq (xis_value_of_expr v) false) ->
+     XJO_red v s v' -> 
+     XJO_red (E_proj1 v) s  (E_proj1 v')
  | XJO_red_proj2 : forall (v v':expr) (s:selectstar),
      (eq (xis_value_of_expr v) true) ->
      (eq (xis_value_of_expr v') true) ->
-     XJO_red (E_apply (E_constant CONST_proj2) (E_pair v v')) s  v' *)
+     XJO_red (E_proj2 (E_pair v v')) s  v'
+ | XJO_red_proj2_eval : forall (v v':expr) (s:selectstar),
+     (eq (xis_value_of_expr v) false) ->
+     XJO_red v s v' -> 
+     XJO_red (E_proj2 v) s  (E_proj2 v') *)
+ 
+ (*| XJO_red_forkeval1 : forall (e e':expr) (s:selectstar) (rl:redlabel) (e'':expr),
+     (eq (xis_value_of_expr e) false) ->
+     XJO_red e s e'' ->
+     XJO_red (E_fork e e') s (E_fork e'' e')
+ | XJO_red_forkeval2 : forall (v e':expr) (s:selectstar) (rl:redlabel) (e'':expr),
+     (eq (xis_value_of_expr v) true) ->
+     (eq (xis_value_of_expr e') false) ->
+     XJO_red e' s e'' ->
+     XJO_red (E_fork v e') s (E_fork v e'')
  | XJO_red_forkmove1 : forall (e e':expr)  (e'':expr) (s:selectstar),
      (eq (xis_value_of_expr e) false) ->
      (eq (xis_value_of_expr e') false) ->
      XJO_red e s e'' ->
-     XJO_red (E_apply  (E_apply (E_constant CONST_fork)  (E_live_expr e) )   (E_live_expr e') ) (Seq S_First s) (E_apply  (E_apply (E_constant CONST_fork)  (E_live_expr e'') )   (E_live_expr e') )
+     XJO_red (E_fork  (E_live_expr e)   (E_live_expr e') ) (Seq S_First s) (E_fork  (E_live_expr e'')   (E_live_expr e') )
  | XJO_red_forkmove2 : forall (e e':expr)  (e'':expr) (s:selectstar),
      (eq (xis_value_of_expr e) false) ->
      (eq (xis_value_of_expr e') false) ->
      XJO_red e' s e'' ->
-     XJO_red (E_apply  (E_apply (E_constant CONST_fork)  (E_live_expr e) )   (E_live_expr e') ) (Seq S_Second s) (E_apply  (E_apply (E_constant CONST_fork)  (E_live_expr e) )   (E_live_expr e'') )
+     XJO_red (E_fork  (E_live_expr e)  (E_live_expr e') ) (Seq S_Second s) (E_fork  (E_live_expr e)    (E_live_expr e'') )
  | XJO_red_forkdeath1 : forall (v e:expr) (s : selectstar),
      (eq (xis_value_of_expr e) true) ->
-     XJO_red (E_apply  (E_apply (E_constant CONST_fork)  (E_live_expr v) )   (E_live_expr e) ) s (E_live_expr  (E_taggingleft   (E_pair v  (E_live_expr e) )  ) )
-(* | XJO_red_forkdeath2 : forall (e v':expr) (s : selectstar),
+     XJO_red (E_fork  (E_live_expr v)    (E_live_expr e) ) s (E_live_expr  (E_taggingleft   (E_pair v  (E_live_expr e) )  ) )
+*) | XJO_red_forkdeath2 : forall (e v':expr) (s : selectstar),
      (eq (xis_value_of_expr v') true) ->
-     XJO_red (E_apply  (E_apply (E_constant CONST_fork)  (E_live_expr e) )   (E_live_expr v') ) s (E_live_expr  (E_taggingright  (E_pair  (E_live_expr e)  v') ) )
+     XJO_red (E_fork  (E_live_expr e)    (E_live_expr v') ) s (E_live_expr  (E_taggingright  (E_pair  (E_live_expr e)  v') ) )
  | XJO_red_context_app1 : forall (e e' e'':expr) (s:selectstar),
      (eq (xis_value_of_expr e) false) ->
      XJO_red e s e'' ->
@@ -139,18 +158,12 @@ Inductive XJO_red : expr -> selectstar -> expr -> Prop :=    (* defn red *)
  | XJO_red_evalcase : forall (e:expr) (x:value_name) (e'':expr) (x':value_name) (e''' e':expr) (s:selectstar),
      (eq (xis_value_of_expr e) false) ->
      XJO_red e s e' ->
-     XJO_red (E_case e x e'' x' e''') s (E_case e' x e'' x' e''')*).  
+     XJO_red (E_case e x e'' x' e''') s (E_case e' x e'' x' e''') .  
 
 
 (*Extraction Relation Fixpoint is_expr_of_expr [1]. *)
 
-Recursive Extraction xis_value_of_expr.
-
-Recursive Extraction select.
-
-Recursive Extraction expr.
-
- Extract Inductive bool => "bool" [ "true" "false" ].
+Extract Inductive bool => "bool" [ "true" "false" ].
 
 Extract Inductive nat => int [ "0" "succ" ] "(fun fO fS n -> if n=0 then fO () else fS (n-1))".
 
@@ -159,6 +172,16 @@ Extract Inductive sumbool => "bool" [ "true" "false" ].
 Extract Inductive list => "list" [ "[]" "(::)" ].
 
 Extract Inductive prod => "(*)"  [ "(,)" ].
+
+Recursive Extraction xis_value_of_expr.
+
+Recursive Extraction subst_expr.
+
+Recursive Extraction select.
+
+Recursive Extraction expr.
+
+ 
 
 Extraction selectstar.
 
