Evaluation/Deleuze/sieve_exec_time.plot
@@ -45,6 +45,21 @@ set term post eps enhanced mono fontfile "/usr/share/texmf/fonts/type1/public/cm
 set output "sieve_mem_bw.eps" 
 replot
 
+unset logscale xy
+set term post eps enhanced color fontfile "/usr/share/texmf/fonts/type1/public/cm-super/sfss1200.pfb" "SFSS1200, 20"
+set output "sieve_ratio_mcon_cont.eps" 
+plot "< paste sieve_cont_data_clean_realtime.txt sieve_mcon_ftt_data_clean_realtime.txt" using 1:($4/$2) with lp title 'mcon_{ftt} vs cont', \
+"< paste sieve_promise_data_clean_realtime.txt sieve_mcon_ftt_data_clean_realtime.txt" using 1:($4/$2) with lp title 'mcon_{ftt} vs promise', \
+"< paste sieve_dlcont_data_clean_realtime.txt sieve_mcon_ftt_data_clean_realtime.txt" using 1:($4/$2) with lp title 'mcon_{ftt} vs dlcont', \
+"< paste sieve_tramp_data_clean_realtime.txt sieve_mcon_ftt_data_clean_realtime.txt" using 1:($4/$2) with lp title 'mcon_{ftt} vs tramp', \
+"< paste sieve_vm_data_clean_realtime.txt sieve_mcon_ftt_data_clean_realtime.txt" using 1:($4/$2) with lp title 'mcon_{ftt} vs vm', \
+"< paste sieve_lwt_data_clean_realtime.txt sieve_mcon_ftt_data_clean_realtime.txt" using 1:($4/$2) with lp title 'mcon_{ftt} vs lwt', \
+"< paste sieve_sys_data_clean_realtime.txt sieve_mcon_ftt_data_clean_realtime.txt" using 1:($4/$2) with lp title 'mcon_{ftt} vs sys'
+
+set term post eps enhanced mono fontfile "/usr/share/texmf/fonts/type1/public/cm-super/sfss1200.pfb" "SFSS1200, 20"
+set output "sieve_ratio_mcon_cont_bw.eps" 
+replot
+
 unset title
 set key top right
 set xlabel 'Last prime < x'
@@ -88,4 +103,18 @@ plot "sieve_cont_opt_opt_data_clean_mem.txt" using 1:2 with lp title 'cont', \
 
 set term post eps enhanced mono fontfile "/usr/share/texmf/fonts/type1/public/cm-super/sfss1200.pfb" "SFSS1200, 20"
 set output "sieve_mem_opt_bw.eps" 
-replotxó
+replot
+
+unset logscale xy
+set term post eps enhanced color fontfile "/usr/share/texmf/fonts/type1/public/cm-super/sfss1200.pfb" "SFSS1200, 20"
+set output "sieve_ratio_mcon_cont_opt.eps" 
+plot "< paste sieve_cont_opt_data_clean_realtime.txt sieve_mcon_ftt_opt_data_clean_realtime.txt" using 1:($4/$2) with lp title 'mcon_{ftt} vs cont', \
+"< paste sieve_promise_opt_data_clean_realtime.txt sieve_mcon_ftt_opt_data_clean_realtime.txt" using 1:($4/$2) with lp title 'mcon_{ftt} vs promise', \
+"< paste sieve_dlcont_opt_data_clean_realtime.txt sieve_mcon_ftt_opt_data_clean_realtime.txt" using 1:($4/$2) with lp title 'mcon_{ftt} vs dlcont', \
+"< paste sieve_tramp_opt_data_clean_realtime.txt sieve_mcon_ftt_opt_data_clean_realtime.txt" using 1:($4/$2) with lp title 'mcon_{ftt} vs tramp', \
+"< paste sieve_lwt_opt_data_clean_realtime.txt sieve_mcon_ftt_opt_data_clean_realtime.txt" using 1:($4/$2) with lp title 'mcon_{ftt} vs lwt', \
+"< paste sieve_sys_opt_data_clean_realtime.txt sieve_mcon_ftt_opt_data_clean_realtime.txt" using 1:($4/$2) with lp title 'mcon_{ftt} vs sys'
+
+set term post eps enhanced mono fontfile "/usr/share/texmf/fonts/type1/public/cm-super/sfss1200.pfb" "SFSS1200, 20"
+set output "sieve_ratio_mcon_cont_opt_bw.eps" 
+replot
